WIP merge extensions

src/tls/Extensions.fsti
@@ -14,199 +14,134 @@ open FStar.Error
 open TLSError
 open TLSConstants
 
-(*************************************************
- Define extension.
- *************************************************)
+(* Extension tag *)
+include Parsers.ExtensionType
 
-// Extensions may (selectively) appear in the following messages
- type ext_msg =
-   | EM_ClientHello
-   | EM_ServerHello
-   | EM_EncryptedExtensions
-   | EM_Certificate
-   | EM_NewSessionTicket
-   | EM_HelloRetryRequest
+(* Server Name Indication *)
+include Parsers.NameType
+include Parsers.ServerName
+include Parsers.ServerNameList
 
-(* As a static invariant, we record that any intermediate, parsed
-   extension and extension lists can be formatted into bytes without
-   overflowing 2^16. This create dependencies on the formatting
-   functions, at odd with recursive extensions. *)
+(* Max fragment length *)
+include Parsers.MaxFragmentLength
 
-(* PRE-SHARED KEYS AND KEY EXCHANGES *)
+(* Certificate Status *)
+include Parsers.CertificateStatusType
+include Parsers.OCSPStatusRequest
+include Parsers.CertificateStatusRequest
+include Parsers.CertificateStatus
 
-type pskIdentity = psk_identifier * PSK.obfuscated_ticket_age
+(* Supported groups *)
+include Parsers.NamedGroup
+include Parsers.NamedGroupList
 
-// used in a refinement below
-val pskiListBytes: list pskIdentity -> bytes
+(* EC point format *)
+include Parsers.ECPointFormat
+include Parsers.ECPointFormatList
 
-// how to build this type without overflows?? 
-noeq type psk =
-  | ClientPSK:
-    // truncated PSK extension, without the list of binder tags.
-    identities: list pskIdentity {let n = length (pskiListBytes identities) in 6 < n /\ n < 65536} ->
-    binders_len: nat {binders_len <= 65535} -> psk
-  | ServerPSK of UInt16.t
-    // index into the client offer's PSK extension
+(* Signature algorithms *)
+include Parsers.SignatureScheme
+include Parsers.SignatureSchemeList
 
-// PSK binders, actually the truncated suffix of TLS 1.3 ClientHello
-// We statically enforce length requirements to ensure that formatting is total.
+(* SRTP *)
+include Parsers.UseSRTPData
 
-//18-02-20 This should be defined in Hashing 
-//18-02-20 We'll need a lemma on HMAC tag lengths. 
-type binder = b:bytes {32 <= length b /\ length b <= 255}
+(* Signed Certificate Timestamp *)
+include Parsers.SignedCertificateTimestampList
 
-(** REMARK: this is more restrictive than in the RFC, which allows up to 2047 binders *)
-type binders =
-  bs:list binder {1 <= List.Tot.length bs /\ List.Tot.length bs < 255}
+(* ALPN *)
+include Parsers.ProtocolName
+include Parsers.ProtocolNameList
 
-// used in HandshakeLog
-val bindersBytes: bs:binders -> b:bytes{length b >= 35 /\ length b <= 65537}
+(* Padding *)
+include Parsers.PaddingExtension
 
-// https://tlswg.github.io/tls13-spec/#rfc.section.4.2.8
-// restricting both proposed PSKs and future ones sent by the server
-// will also be used in the PSK table, and possibly in the configs
-type psk_kex =
-  | PSK_KE
-  | PSK_DHE_KE
+(* Ticket *)
+include Parsers.SessionTicket
 
-type client_psk_kexes = l:list psk_kex
-  { l = [PSK_KE] \/ l = [PSK_DHE_KE] \/ l = [PSK_KE; PSK_DHE_KE] \/ l = [PSK_DHE_KE; PSK_KE] }
+(* EDI (NewSessionTicket) *)
+include Parsers.EarlyDataIndicationNewSessionTicket
 
-#set-options "--admit_smt_queries true"
-let client_psk_kexes_length (l:client_psk_kexes): Lemma (List.Tot.length l < 3) = ()
+(* Heartbeat *)
+include Parsers.HeartbeatMode
+include Parsers.HeartbeatExtension
 
-(* EARLY DATA INDICATION *)
+(* Pre-shared key *)
+include Parsers.PskIdentity
+include Parsers.PskBinderEntry
+include Parsers.OfferedPsks
+include Parsers.PreSharedKeyServerExtension
 
-type earlyDataIndication = option UInt32.t // Some max_early_data_size, only in NewSessionTicket
+(* Key exchange mode *)
+include Parsers.PskKeyExchangeMode
+include Parsers.PskKeyExchangeModes
 
-(* EC POINT FORMATS *)
+(* Supported version *)
+include Parsers.ProtocolVersion
+include Parsers.SupportedVersions
 
-type point_format =
-  | ECP_UNCOMPRESSED
-  | ECP_UNKNOWN of (n:nat{repr_bytes n <= 1})
+(* Cookie *)
+include Parsers.Cookie
 
-// Move TLSConstants?
-val alpnBytes : alpn -> b:bytes{length b < 65536}
+(* Certificate type *)
+include Parsers.CertificateType
+include Parsers.ClientCertTypeExtension
+include Parsers.ServerCertTypeExtension
 
-// The length exactly reflects the RFC format constraint <2..254>
-type protocol_versions =
-  | ServerPV of protocolVersion
-  | ClientPV of l:list protocolVersion' {0 < List.Tot.length l /\ List.Tot.length l < 128}
+(* Certificate Authorities *)
+include Parsers.CertificateAuthoritiesExtension
 
-// We constrain unknown extensions to have headers different from
-// known extensions; we rely on parametricity to avoid recursion
-// between the datatype and its formatting property.
-type unknownTag = lbytes 2 -> Type0
+(* OID filter *)
+include Parsers.OIDFilterExtension
 
-// ExtensionType and Extension Table in https://tlswg.github.io/tls13-spec/#rfc.section.4.2.
-// M=Mandatory, AF=mandatory for Application Features in https://tlswg.github.io/tls13-spec/#rfc.section.8.2.
-noeq type extension' (p: unknownTag) =
-  | E_server_name of list serverName (* M, AF *) (* RFC 6066 *)
-  | E_supported_groups of list CommonDH.namedGroup (* M, AF *) (* RFC 7919 *)
-  | E_signature_algorithms of signatureSchemeList (* M, AF *) (* RFC 5246 *)
-  | E_signature_algorithms_cert of signatureSchemeList (* TLS 1.3#23 addition; TLS 1.2 should also support it *)
-  | E_key_share of CommonDH.keyShare (* M, AF *)
-  | E_pre_shared_key of psk (* M, AF *)
-  | E_session_ticket of bytes
-  | E_early_data of earlyDataIndication
-  | E_supported_versions of protocol_versions   (* M, AF *)
-  | E_cookie of b:bytes {0 < length b /\ length b < 65536}  (* M *)
-  | E_psk_key_exchange_modes of client_psk_kexes (* client-only; mandatory when proposing PSKs *)
-  | E_extended_ms
-  | E_ec_point_format of list point_format
-  | E_alpn of alpn
-  | E_unknown_extension: x: lbytes 2 {p x} -> bytes -> extension' p (* header, payload *)
-(*
-We do not yet support the extensions below (authenticated but ignored)
-  | E_max_fragment_length
-  | E_status_request
-  | E_use_srtp
-  | E_heartbeat
-  | E_signed_certifcate_timestamp
-  | E_client_certificate_type
-  | E_server_certificate_type
-  | E_certificate_authorities
-  | E_oid_filters
-  | E_post_handshake_auth
-  | E_renegotiation_info of renegotiationInfo
-*)
+(* Key share *)
+include Parsers.UncompressedPointRepresentation32
+include Parsers.UncompressedPointRepresentation48
+include Parsers.UncompressedPointRepresentation66
+include Parsers.MontgomeryPoint32
+include Parsers.MontgomeryPoint56
+include Parsers.ServerDHParams
+include Parsers.KeyShareEntry
+include Parsers.KeyShareClientHello
 
+(* Unknown *)
+include Parsers.UnknownExtension
 
+(* New Session Ticket *)
+include Parsers.NewSessionTicketExtension
+include Parsers.NewSessionTicketExtensions
 
-val bindersLen: #p: unknownTag -> el: list (extension' p) -> nat
-val string_of_extension: #p: unknownTag -> extension' p -> string
-val string_of_extensions: #p: unknownTag -> list (extension' p) -> string
+(* Certificate Request *)
+include Parsers.CertificateRequestExtension
+include Parsers.CertificateRequestExtensions
 
-(** shallow equality, comparing just the extension tags *)
-val sameExt: #p: unknownTag -> e1: extension' p -> e2: extension' p -> bool
+(* Certificate *)
+include Parsers.CertificateExtension
+include Parsers.CertificateExtensions
 
-(*************************************************
- extension formatting
- *************************************************)
+(* Encrypted Extension *)
+include Parsers.EncryptedExtension
+include Parsers.EncryptedExtensions
 
-val unknown: unknownTag
-val is_unknown: x: lbytes 2 -> b:bool {b2t b <==> unknown x}
-type extension = extension' unknown
+(* Hello Retry Request *)
+include Parsers.HRRExtension
+include Parsers.HRRExtensions
+
+(* Server Hello *)
+include Parsers.ServerHelloExtension
+include Parsers.ServerHelloExtensions
+
+(* Client Hello *)
+include Parsers.ClientHelloExtension
+include Parsers.ClientHelloExtensions
 
 // TLSConstants defines the application-level type for custom extensions
-val ext_of_custom: custom_extensions -> list extension
-val custom_of_ext: list extension -> custom_extensions
-val app_ext_filter: option (list extension) -> option (list extension)
+val cext_of_custom: custom_extensions -> clientHelloExtensions
+val eext_of_custom: custom_extensions -> encryptedExtensions
+val custom_of_cext: clientHelloExtensions -> custom_extensions
+val custom_of_eext: encryptedExtensions -> custom_extensions
 
-let encryptedExtension (ext: extension) : bool =
-  match ext with
-  | E_server_name _
-  | E_supported_groups _
-  | E_alpn _
-  | E_unknown_extension _ _
-  | E_early_data _ -> true
-  | _ -> false
-
-(** Serializes an extension *)
-val extensionBytes: ext:extension -> b:bytes { 2 <= length b /\ length b < 65536 }
-val extensionBytes_is_injective:
-  ext1: extension -> s1: bytes{ UInt.size (length (extensionBytes ext1) + length s1) UInt32.n } ->
-  ext2: extension -> s2: bytes{ UInt.size (length (extensionBytes ext2) + length s2) UInt32.n } -> 
-  Lemma
-  (requires (extensionBytes ext1 @| s1 = extensionBytes ext2 @| s2))
-  (ensures  (ext1 == ext2 /\ s1 == s2))
-
-// we'll need to reveal more to build extensions...
-val extensionListBytes: exts: list extension -> bytes
-type extensions = exts:list extension {repr_bytes (length (extensionListBytes exts)) <= 2}
-
-(** Serializes a list of extensions.
-  If there is a PreSharedKey client extension, then add the length of the PSK binders to
-  the total length. Note that the `E_pre_shared_key` argument includes the length of
-  binders in this case.
-*)
-
-type valid_extensions = exts: extensions {length (extensionListBytes exts) + bindersLen exts < 65536}
-
-val extensionsBytes:
-  exts:valid_extensions -> b:bytes {2 <= length b /\ length b < 2 + 65536}
-
-val extensionsBytes_is_injective_strong:
-  exts1:valid_extensions -> s1: bytes{ UInt.size (length (extensionsBytes exts1) + length s1) UInt32.n } ->
-  exts2:valid_extensions -> s2: bytes{ UInt.size (length (extensionsBytes exts2) + length s2) UInt32.n } -> Lemma
-  (requires extensionsBytes exts1 @| s1 = extensionsBytes exts2 @| s2)
-  (ensures exts1 == exts2 /\ s1 == s2)
-
-val extensionsBytes_is_injective:
-  ext1:valid_extensions ->
-  ext2:valid_extensions -> Lemma
-  (requires Bytes.equal (extensionsBytes ext1) (extensionsBytes ext2))
-  (ensures ext1 == ext2)
-
-(*************************************************
- Extension parsing
-**************************************************)
-
-val parseExtension:     ext_msg -> bytes -> result (extension * option binders)
-val parseExtensions:    ext_msg -> bytes -> result (extensions * option binders)
-
-(** Called by HandshakeMessages; returns either Some,Some or None; why not using extensions here too? *)
-val parseOptExtensions: ext_msg -> bytes -> result (option (list extension) * option binders)
+val bindersLen: clientHelloExtensions -> nat
 
 (*************************************************
  Other extension functionality
@@ -220,27 +155,25 @@ val prepareExtensions:
   protocolVersion ->
   k:valid_cipher_suites{List.Tot.length k < 256} ->
   option bytes -> // SNI
-  option alpn -> // ALPN
+  option protocolNameList -> // ALPN
   custom_extensions -> // application-handled extensions
   bool -> // EMS
   bool ->
   bool -> // EDI (Nego checks that PSK is compatible)
   option bytes -> // session_ticket
   signatureSchemeList ->
-  //18-02-26 
-  // list CommonDH.namedGroup -> // FIXME: was: list valid_namedGroup, but the latter type disappeared
   list CommonDH.supportedNamedGroup ->
   option (cVerifyData * sVerifyData) ->
-  option CommonDH.keyShare ->
+  option CommonDH.keyShareEntry ->
   list (PSK.pskid * pskInfo) ->
   now: UInt32.t -> // for obfuscated ticket age
-  l:list extension{List.Tot.length l < 256}
+  clientHelloExtensions
 
 val negotiateClientExtensions:
   protocolVersion ->
   config ->
-  option (list extension) ->
-  option (list extension) ->
+  clientHelloExtensions ->
+  serverHelloExtensions ->
   cipherSuite ->
   option (cVerifyData * sVerifyData) ->
   bool ->
@@ -248,15 +181,15 @@ val negotiateClientExtensions:
 
 val negotiateServerExtensions:
   protocolVersion ->
-  option (list extension) ->
+  clientHelloExtensions ->
   list cipherSuiteName ->
   config ->
   cipherSuite ->
   option (cVerifyData * sVerifyData) ->
   option nat ->
-  option CommonDH.keyShare ->
+  option CommonDH.keyShareEntry ->
   bool ->
-  result (option (list extension))
+  result (serverHelloExtensions * encryptedExtensions)
 
 val default_signatureScheme:
   protocolVersion -> cipherSuite -> HyperStack.All.ML signatureSchemeList
